src/BatchOperations/Specs.v
@@ -1,0 +1,385 @@
+Require Import String Omega.
+Require Import Primitives Layer1.
+Require Import BatchOperations.Definitions.
+
+Theorem encrypt_all_ok :
+  forall vl k o d a,
+    let kl := fst (fst a) in
+    let em := snd (fst a) in
+    let hm := snd a in
+    << o, d, a >>
+    ([[ consistent_with_upds em
+             (map (encrypt k) vl) (map (fun v=> (k,v)) vl) ]])
+      (encrypt_all k vl)
+    << r, ar >>
+      ([[ r = map (encrypt k) vl ]] *
+       [[ ar = (kl, upd_batch em r (map (fun v => (k, v)) vl), hm) ]])%pred
+      ([[ exists n, ar = (kl, upd_batch em (firstn n (map (encrypt k) vl)) (map (fun v => (k, v)) (firstn n vl)), hm) ]]).
+Proof.
+  induction vl; do 5 intro; cleanup.
+  {
+    eapply pre_impl.
+    eapply post_impl.
+    eapply crash_impl.
+    apply ret_ok.
+    intros; cancel.
+    exists 0; simpl; eauto.
+    intros; cancel.
+    simpl; cancel.
+  }
+
+  {
+    cleanup. destruct a0, p.
+    simpl encrypt_all; simpl fst; simpl snd.
+    eapply bind_ok.
+    { intros; eapply pre_impl; [ apply (@encrypt_ok _ _ _ k a) |intros; simpl in *; cancel]. }
+    { intros; simpl. instantiate(1:= fun _ => emp); simpl; cancel. }
+    { intros; simpl; cancel; exists 0; simpl; eauto. }
+    
+    intros; cleanup.
+    eapply bind_ok.
+    { intros; eapply pre_impl; try apply IHvl.
+      intros; simpl in *.
+      repeat destruct_lifts; cleanup; cancel. }
+    { intros; simpl in *; cancel.
+      instantiate (1:= fun _ => emp); simpl; cancel.  }
+    { intros; simpl in *; repeat destruct_lifts; cleanup;
+      simpl; cancel; simpl; exists (S n); eauto. }
+    { intros.
+      eapply pre_impl.
+      eapply post_impl.
+      eapply crash_impl.
+      apply ret_ok.
+      { intros; cancel.
+        simpl in *; repeat destruct_lifts; cleanup.
+        exists (S (length vl)); simpl.
+        rewrite firstn_map_comm.
+        rewrite firstn_exact; eauto. }
+      { intros; simpl in *; repeat destruct_lifts; cleanup; cancel. }
+      { intros; simpl; cancel. }
+    }
+  }
+Qed.
+
+Lemma get_all_existing_length_le:
+  forall A AEQ V (m: @mem A AEQ V) al,
+    length (get_all_existing m al) <= length al.
+Proof.
+  induction al; intros; simpl in *; eauto.
+  destruct (m a); simpl in *; eauto.
+  omega.
+Qed.
+
+Theorem decrypt_all_ok :
+  forall evl k o d a,
+    let kl := fst (fst a) in
+    let em := snd (fst a) in
+    let hm := snd a in
+    let kvl := get_all_existing em evl in
+    let vl := map snd kvl in
+    << o, d, a >>
+    ([[ evl = map (encrypt k) vl ]] *
+     [[ repeat k (length evl) = map fst kvl ]])
+      (decrypt_all k evl)
+    << r, ar >>
+      ([[ r = vl ]] *
+       [[ ar = a ]])%pred
+      ([[ ar = a ]]).
+Proof.
+  induction evl; intros; cleanup.
+  {
+    eapply pre_impl.
+    eapply post_impl.
+    eapply crash_impl.
+    apply ret_ok.
+    all: intros; cancel.
+  }
+
+  {
+    cleanup. destruct a0, p.
+    destruct_fresh (m a).
+    {
+      destruct p.
+      simpl decrypt_all; simpl fst; simpl snd.
+      eapply bind_ok.
+      { intros; eapply pre_impl; [ apply (@decrypt_ok _ _ _ k a) |intros; simpl in *; cancel].
+        cleanup; simpl in *.
+        inversion H2; eauto.
+        cleanup; simpl in *.
+        inversion H2; inversion H3; eauto. }
+      { intros; simpl. instantiate(1:= fun _ => emp); simpl; cancel. }
+      { intros; simpl; cancel. }
+      
+      intros; cleanup.
+      eapply bind_ok.
+      { intros; eapply pre_impl; try apply IHevl.
+        intros; simpl in *.
+        repeat destruct_lifts; cleanup; cancel. }
+      { intros; simpl in *; cancel.
+        instantiate (1:= fun _ => emp); simpl; cancel.  }
+      { intros; simpl in *; repeat destruct_lifts; cleanup;
+        simpl; cancel. }
+
+      intros.
+      eapply pre_impl.
+      eapply post_impl.
+      eapply crash_impl.
+      apply ret_ok.
+      { intros; cancel.
+        simpl in *; repeat destruct_lifts; cleanup; eauto. }
+      { intros; simpl in *; repeat destruct_lifts; cleanup; cancel. }
+      { intros; simpl; cancel. }
+    }
+    
+    {
+      unfold hoare_triple; intros.
+      destruct_lifts; cleanup.
+      assert (A: length (a :: evl) =
+        length (map (encrypt k)
+                    (map snd (get_all_existing m evl))))
+        by (cleanup; eauto).
+      simpl in A.
+      repeat rewrite map_length in A.
+      pose proof (@get_all_existing_length_le _ _ _ m evl).
+      omega.
+    }
+  }
+Qed.
+
+Lemma firstn_rolling_hash_list_comm:
+  forall n h vl,
+    firstn n (rolling_hash_list h vl) = rolling_hash_list h (firstn n vl).
+Proof.
+  induction n; intros; simpl in *; eauto.
+  destruct vl; simpl; eauto.
+  rewrite IHn; eauto.
+Qed.
+
+Lemma firstn_hash_and_pair_comm:
+  forall n h vl,
+    firstn n (hash_and_pair h vl) = hash_and_pair h (firstn n vl).
+Proof.
+  induction n; intros; simpl in *; eauto.
+  destruct vl; simpl; eauto.
+  rewrite IHn; eauto.
+Qed.
+
+Theorem hash_all_ok :
+  forall vl h o d a,
+    let kl := fst (fst a) in
+    let em := snd (fst a) in
+    let hm := snd a in
+    let rhl := rolling_hash_list h vl in
+    let hvl := hash_and_pair h vl in
+    << o, d, a >>
+    ([[ consistent_with_upds hm rhl hvl ]])
+      (hash_all h vl)
+    << r, ar >>
+      ([[ r = rolling_hash h vl ]] *
+       [[ ar = (kl, em, upd_batch hm rhl hvl) ]])%pred
+      ([[ exists n, ar = (kl, em, upd_batch hm (firstn n rhl) (firstn n hvl)) ]]).
+Proof.
+  induction vl; intros; cleanup.
+  {
+    eapply pre_impl.
+    eapply post_impl.
+    eapply crash_impl.
+    apply ret_ok.
+    intros; cancel.
+    exists 0; simpl; eauto.
+    intros; cancel.
+    simpl; cancel.
+  }
+
+  {
+    cleanup. destruct a0, p.
+    simpl hash_all; simpl fst; simpl snd.
+    eapply bind_ok.
+    { intros; eapply pre_impl; [ apply (@hash_ok _ _ _ h a) |intros; simpl in *; cancel]. }
+    { intros; simpl. instantiate(1:= fun _ => emp); simpl; cancel. }
+    { intros; simpl; cancel; exists 0; simpl; eauto. }
+  
+    intros; cleanup.
+    eapply bind_ok.
+    { intros; eapply pre_impl; try apply IHvl.
+      intros; simpl in *.
+      repeat destruct_lifts; cleanup; cancel. }
+    { intros; simpl in *; cancel.
+      instantiate (1:= fun _ => emp); simpl; cancel.  }
+    { intros; simpl in *; repeat destruct_lifts; cleanup;
+      simpl; cancel; simpl; exists (S n); eauto. }
+
+    { intros.
+      eapply pre_impl.
+      eapply post_impl.
+      eapply crash_impl.
+      apply ret_ok.
+      { intros; cancel.
+        simpl in *; repeat destruct_lifts; cleanup.
+        exists (S (length vl)); simpl.
+        rewrite firstn_rolling_hash_list_comm.
+        rewrite firstn_hash_and_pair_comm.
+        rewrite firstn_exact; eauto. }
+      { intros; simpl in *; repeat destruct_lifts; cleanup; cancel. }
+      { intros; simpl; cancel. }
+    }
+  }
+Qed.
+
+Theorem read_consecutive_ok :
+  forall n start vl o d a,
+    << o, d, a >>
+      (start |=> vl *
+      [[ length vl = n ]])
+      (read_consecutive start n)
+    << r, ar >>
+      (start |=> vl *
+       [[ r = map fst vl ]] *
+       [[ ar = a ]])%pred
+      (start |=> vl *
+      [[ ar = a ]]).
+Proof.
+  induction n; intros; cleanup.
+  {
+    eapply post_impl.
+    eapply crash_impl.
+    eapply pre_impl.
+    apply ret_ok.
+    all: simpl in *; intros; repeat destruct_lifts; cancel.
+    all: match goal with
+         |[H: length _ = 0 |- _] =>
+          apply length_zero_iff_nil in H
+         end; cleanup; simpl; eauto.
+  }
+
+  {
+    cleanup.
+    destruct vl.
+    {
+      unfold hoare_triple; simpl; intros.
+      repeat destruct_lifts; congruence.
+    }
+    
+    simpl read_consecutive; simpl fst; simpl snd.
+    eapply bind_ok.
+    { intros; eapply pre_impl.
+      eapply add_frame; apply (@read_ok _ _ start).
+      simpl; cancel.
+    }
+    { intros; simpl.
+      instantiate (1:= fun ar => start |=> (d0::vl)); simpl; cancel. }
+    { intros; simpl; cancel. }
+    
+    intros; cleanup.
+      eapply bind_ok.
+      { intros; eapply pre_impl.
+        eapply add_frame; try apply IHn.
+        intros; simpl in *.
+        repeat destruct_lifts; cleanup; cancel.
+        eassign vl; cancel.
+        destruct_lift H; cleanup; eauto.
+      }
+      { intros; simpl in *; cancel.
+        instantiate (1:= fun _ => start |=> (d0::vl)); simpl; cancel.  }
+      { intros; simpl in *; repeat destruct_lifts; cleanup;
+        simpl; cancel.
+      destruct_lift H0; eauto. }
+
+      intros.
+      eapply pre_impl.
+      eapply post_impl.
+      eapply crash_impl.
+      eapply add_frame.
+      apply ret_ok.
+      { intros; cancel.
+        simpl in *; destruct_lift H;
+        destruct_lift H0; destruct_lift H2;
+        cleanup; eauto. }
+      { intros; simpl in *; destruct_lift H;
+        destruct_lift H0; destruct_lift H2;
+        cleanup; cancel. }
+      { intros; simpl; cancel. }
+    }
+Qed.
+
+Definition vsupd {V} (v: V) (vs: V * list V) := (v, fst vs::snd vs).
+
+Fixpoint map_pointwise {A B} (fl : list (A -> B)) (al : list A) :=
+  match fl, al with
+  | f::fl', a::al' =>
+    (f a)::map_pointwise fl' al'
+  | _, _ => nil
+  end.
+
+Theorem write_consecutive_ok :
+  forall vl start vsl o d a,
+    << o, d, a >>
+      (start |=> vsl *
+      [[ length vsl = length vl ]])
+      (write_consecutive start vl)
+    << r, ar >>
+      (start |=> (map_pointwise (map vsupd vl) vsl) *
+       [[ ar = a ]])%pred
+      (exists* n, start |=> (map_pointwise (map vsupd (firstn n vl)) (firstn n vsl)) *
+            (start + n) |=> skipn n vsl *  
+      [[ ar = a ]]).
+Proof.
+  unfold vsupd; induction vl; intros; cleanup.
+  {
+    eapply post_impl.
+    eapply crash_impl.
+    eapply pre_impl.
+    apply ret_ok.
+    all: simpl in *; intros; repeat destruct_lifts; cancel.
+    all: match goal with
+         |[H: length _ = 0 |- _] =>
+          apply length_zero_iff_nil in H
+         end; cleanup; simpl; eauto.
+    rewrite firstn_nil, skipn_nil; simpl.
+    cancel.
+  }
+
+  {
+    cleanup.
+    destruct vsl.
+    {
+      unfold hoare_triple; simpl; intros.
+      repeat destruct_lifts; congruence.
+    }
+    
+    simpl write_consecutive; simpl fst; simpl snd.
+    eapply bind_ok.
+    { intros; eapply pre_impl.
+      eapply add_frame; apply write_ok.
+      simpl; cancel.
+    }
+    { intros; simpl.
+      instantiate (1:= fun ar => S start |=> vsl * start |-> (a, fst d0 :: snd d0)); simpl; cancel. }
+    { intros; simpl; cancel.
+      eassign 0; simpl; cancel.
+      rewrite Nat.add_0_r; cancel. }
+    
+
+      intros.
+      eapply pre_impl.
+      eapply post_impl.
+      eapply crash_impl.
+      eapply add_frame.
+      apply IHvl.
+      { intros; cancel.
+        eassign (S n); eassign vsl; simpl.
+        rewrite Nat.add_succ_r; cancel.
+        simpl in *; destruct_lift H;
+        destruct_lift H0; destruct_lift H2;
+        cleanup; eauto. }
+      { intros; simpl in *; destruct_lift H;
+        destruct_lift H0; destruct_lift H2;
+        cleanup; cancel. }
+      { intros; simpl in *; destruct_lift H;
+        destruct_lift H0; destruct_lift H2;
+        cleanup; cancel. }
+      Unshelve.
+      eauto.
+    }
+Qed.
+
